Core/Examples/Boolean.lean
@@ -20,7 +20,7 @@ not = λ x → case x of
 -/
 def notTerm : Term := λ[ .global "Bool" ]
   match! #0
-         v[ "True", "False" ]
+         v[ g#"True", g#"False" ]
          v[
          g# "False",
          g# "True" ]
@@ -36,9 +36,9 @@ def notTerm : Term := λ[ .global "Bool" ]
  -/
 def eqBool : Term := λ[ .global "Bool" ] λ[ .global "Bool" ]
   match! #1
-   v[ "True", "False" ]
-   v[ match! #0 v[ "True", "False" ] v[ g#"True", g#"False"] ,
-      match! #0 v[ "True", "False" ] v[ g# "False", g# "False"]
+   v[ g#"True", g#"False" ]
+   v[ match! #0 v[ g#"True", g#"False" ] v[ g#"True", g#"False"] ,
+      match! #0 v[ g#"True", g#"False" ] v[ g# "False", g# "False"]
     ]
 
 
